src/impl/TLS13.Impl.Driver.Pairing.fsti
@@ -253,10 +253,21 @@ let client_server_driver_supported_profile_state_inputs
   (server:CS.connection_state)
   : prop =
   CS.paired_x25519_key_shares client server /\
-  CS.connection_supported_profile_key_schedule_lineage client /\
-  CS.connection_supported_profile_key_schedule_lineage server /\
   CS.paired_handshake_events client server /\
   CS.supported_profile_all_record_material_inputs_agree client server
+
+val lemma_client_server_driver_supported_profile_key_material_inputs_agree
+  (client:CS.connection_state)
+  (server:CS.connection_state)
+  : Lemma
+      (requires
+        CD.client_driver_application_ready client /\
+        SD.server_driver_application_ready server /\
+        client_server_driver_supported_profile_state_inputs client server)
+      (ensures
+        CS.supported_profile_client_server_key_material_inputs_agree
+          client
+          server)
 
 noextract
 let client_server_driver_key_material_no_read_ahead_component_inputs
